ml_sources/examples/crdt/statelib/examples/grow_only_set/grow_only_set_code.ml
@@ -10,10 +10,6 @@ let mutator : ('a, 'stTy) mutatorFnTy =
   fun (_i : int) (gs : 'stTy) (op : 'a) ->
   set_add op gs
 
-(* TODO: move to the aneris lib. *)
-let set_union (s1 : 'a aset) (s2 : 'a aset) : 'a aset =
-  set_foldl (fun su e -> set_add e su) s1 s2
-
 let merge (st1 : 'a stTy) (st2 : 'a stTy) : 'a stTy =
   set_union st1 st2
 
