aneris/aneris_lang/lib/serialization/serialization_proof.v
@@ -1,7 +1,7 @@
 From iris.algebra Require Import gmap.
 From aneris.prelude Require Import misc.
 From aneris.aneris_lang Require Import lang proofmode.
-From aneris.aneris_lang.lib Require Import network_util_proof assert_proof.
+From aneris.aneris_lang.lib Require Import inject list_proof network_util_proof assert_proof.
 From aneris.aneris_lang.lib Require Export serialization_code.
 
 Record serialization := {
@@ -84,7 +84,7 @@ Definition bool_to_int (b : bool) := if b then 1 else 0.
 Definition bool_valid_val (v : val) := ∃ (b : bool), v = #b.
 
 Definition bool_ser_str (b : bool) : string :=
-  StringOfZ $ bool_to_int b.
+  StringOfZ (bool_to_int b).
 
 Definition bool_is_ser (v : val) (s : string) :=
   ∃ (b : bool), v = #b ∧ s = bool_ser_str b.
@@ -113,7 +113,7 @@ Lemma bool_deser_spec `{!anerisG Mdl Σ} ip v s :
 Proof.
   iIntros (Φ [b [-> ->]]) "HΦ".
   rewrite /bool_deser /bool_is_ser. wp_pures.
-  assert (un_op_eval IntOfString #(StringOfZ $ bool_to_int b) =
+  assert (un_op_eval IntOfString #(StringOfZ (bool_to_int b)) =
           Some (InjRV #(bool_to_int b))).
   { rewrite /= ZOfString_inv //=. }
   by destruct b; wp_pures; iApply "HΦ".
@@ -570,6 +570,159 @@ Section option_serialization.
 
 End option_serialization.
 
+Section list_serialization.
+
+  Context (E : serialization).
+  Context `{!Inject A val}.
+
+
+  Definition list_valid_val (v : val) :=
+    ∃ (la: list A), is_list la v ∧ (∀ x, x ∈ la → s_valid_val E $ x).
+
+  Fixpoint list_is_ser_aux (la : list A) (s : string) :=
+    match la with
+      | hd :: tl =>
+          ∃ s1 s2 : string,
+            E.(s_is_ser) $hd s1 ∧
+            s = prod_ser_str s1 s2 ∧
+            list_is_ser_aux tl s2
+      | [] => s = ""
+  end.
+
+  Definition list_is_ser (v : val) (s : string) :=
+    ∃ (l : list A), is_list l v ∧ list_is_ser_aux l s.
+
+  Lemma list_is_ser_aux_valid_val l :
+    ∀ s x, list_is_ser_aux l s → x ∈ l → s_valid_val E $ x.
+  Proof.
+    induction l as [|a' l']; first by set_solver.
+    intros ?? (?&?&?&?&?) [->|Hin]%elem_of_cons;
+      by [eapply s_is_ser_valid| eapply IHl'].
+  Qed.
+
+  Lemma list_is_ser_valid (v : val) (s : string) :
+    list_is_ser v s -> list_valid_val v.
+  Proof.
+    destruct 1 as (l&Hl&Hs).
+    exists l. split; first done.
+    intros x Hx. by eapply list_is_ser_aux_valid_val.
+  Qed.
+
+  Lemma list_ser_spec `{!anerisG Mdl Σ} ip v:
+    {{{ ⌜list_valid_val v⌝ }}}
+      (list_serializer (s_serializer E)).(s_ser) v @[ip]
+    {{{ (s : string), RET #s; ⌜list_is_ser v s⌝ }}}.
+  Proof.
+    iIntros (Φ) "Hv HΦ".
+    iLöb as "IH" forall (Φ v).
+    wp_rec.
+    iDestruct "Hv" as %(l&Hvl&Hvv).
+    destruct l as [|a l].
+    - rewrite Hvl.
+      wp_pures.
+      iApply "HΦ".
+      iPureIntro.
+      rewrite /list_is_ser; eexists []; done.
+    - simpl in Hvl, Hvv.
+      destruct Hvl as [lv [-> Hvl]].
+      wp_pures.
+      wp_apply (s_ser_spec E).
+      { iPureIntro.
+        apply Hvv.
+        set_solver. }
+      iIntros (s1) "%Hs1".
+      wp_pures.
+      wp_bind (list_ser (s_ser (s_serializer E)) _).
+      iApply "IH"; [iPureIntro; exists l; set_solver |].
+      iIntros "!>" (s2) "%Hs2".
+      wp_pures.
+      destruct Hs2 as (l'& Hs2x & Hs2y).
+      iApply "HΦ".
+      iPureIntro.
+      exists (a :: l').
+      split; first by eexists.
+      by exists s1, s2.
+  Qed.
+
+  Lemma list_deser_spec `{!anerisG Mdl Σ} ip v s:
+    {{{ ⌜list_is_ser v s⌝ }}}
+      (list_serializer (s_serializer E)).(s_deser) #s @[ip]
+      {{{ RET v; True }}}.
+  Proof.
+    iIntros (Φ) "Hs HΦ".
+    iLöb as "IH" forall (Φ v s).
+    wp_rec.
+    iDestruct "Hs" as %(l & Hl1 & Hl2).
+    destruct l as [|a l]; simpl.
+    - rewrite Hl1 Hl2.
+      wp_find_from; first by split_and!; [|by apply nat_Z_eq; first lia].
+      wp_pures.
+      by iApply "HΦ".
+    - destruct Hl1 as [lv [-> Hl1]].
+      destruct Hl2 as (s1&s2&Hs1&->&Hl2).
+      rewrite! /prod_ser_str.
+      wp_find_from; first by split_and!; [|by apply nat_Z_eq; first lia].
+      erewrite (index_0_append_char ); auto; last first.
+      { apply valid_tag_stringOfZ. }
+      wp_pures.
+      wp_substring; first by split_and!; [|by apply nat_Z_eq; first lia|done].
+      rewrite substring_0_length_append.
+      wp_pure _.
+      { simpl. rewrite ZOfString_inv //. }
+      wp_apply wp_unSOME; [done|].
+      iIntros "_ /=". wp_pures.
+      wp_substring;
+        first by split_and!;
+              [|by apply nat_Z_eq; first lia|by apply nat_Z_eq; first lia].
+      replace (Z.to_nat (Z.add (Z.of_nat
+                                  (String.length
+                                     (StringOfZ (Z.of_nat (String.length s1)))))
+                               1%Z)) with
+        (String.length (StringOfZ (Z.of_nat (String.length s1))) + 1)%nat by lia.
+      replace (Z.to_nat (String.length s1)) with (String.length s1)%nat by lia.
+      rewrite substring_add_length_app /= substring_0_length_append.
+      wp_pures.
+      rewrite !length_app /=.
+      match goal with
+      | |- context [Substring _ _ ?X] =>
+          replace X with (Val #(String.length s2)); last first
+      end.
+    { repeat f_equal; lia. }
+    wp_substring; first by split_and!; [|by apply nat_Z_eq; first lia|done].
+    match goal with
+    | |- context [substring ?X _ _] =>
+      replace X with (String.length
+                        (StringOfZ (Z.of_nat (String.length s1))) + 1 +
+                        String.length s1)%nat by lia
+    end.
+    rewrite -plus_assoc substring_add_length_app /= substring_length_append.
+    wp_pures.
+    wp_apply (s_deser_spec E); first done.
+    iIntros "_"; simpl.
+    wp_pures.
+    wp_bind (list_deser _ _).
+    iApply ("IH" $! _ lv); first by iPureIntro; eexists.
+    iIntros "!> _".
+    wp_pures.
+    wp_apply (wp_list_cons _ l); first done.
+    iIntros (v Hl).
+    assert ((InjRV ($ a, lv) = v)) as ->.
+    { destruct Hl as [lv' [-> Hl1']].
+      by rewrite (is_list_eq _ _ _ Hl1 Hl1'). }
+    by iApply "HΦ".
+  Qed.
+
+Definition list_serialization : serialization :=
+  {| s_valid_val := list_valid_val;
+     s_serializer := list_serializer E.(s_serializer);
+     s_is_ser := list_is_ser;
+     s_is_ser_valid := list_is_ser_valid;
+     s_ser_spec := @list_ser_spec;
+     s_deser_spec := @list_deser_spec; |}.
+
+End list_serialization.
+
+
 (* Recursively destructs the definition of the argument hypothesis of the shape
    [H : *_is_ser] *)
 Ltac destruct_is_ser H :=
@@ -586,5 +739,6 @@ Ltac destruct_is_ser H :=
   | option_is_ser _ _ _ =>
     destruct H as (?&?& [(? & ?Hl & ?)|(? & ?Hr & ?)]);
     [destruct_is_ser Hl | destruct_is_ser Hr]
+  | list_is_ser _ _ _ _ => destruct H as (?&?&?)
   | _ => idtac
   end; simplify_eq.
